src/PredCrash.v
@@ -149,14 +149,26 @@ Lemma possible_crash_upd : forall m m' a v vs,
   possible_crash (upd m a vs) (upd m' a (v, nil)).
 Proof.
   unfold possible_crash; intuition.
+  destruct (addr_eq_dec a a0); subst.
+  repeat rewrite upd_eq; auto.
+  specialize (H a0); intuition; right; eexists; eauto.
+  repeat rewrite upd_ne; auto.
+Qed.
+
+Lemma possible_crash_updSome : forall m m' a v vs,
+  possible_crash m m' ->
+  In v (vsmerge vs) ->
+  possible_crash (updSome m a vs) (updSome m' a (v, nil)).
+Proof.
+  unfold possible_crash; intuition.
   pose proof (H a) as H'; intuition; repeat deex.
 
-  - repeat rewrite upd_none by eauto.
+  - repeat rewrite updSome_none by eauto.
     intuition.
 
   - destruct (addr_eq_dec a a0); subst.
-    + repeat erewrite upd_eq by eauto. right. eauto.
-    + repeat rewrite upd_ne by eauto. eauto.
+    + repeat erewrite updSome_eq by eauto. right. eauto.
+    + repeat rewrite updSome_ne by eauto. eauto.
 Qed.
 
 Definition synced_mem (m : rawdisk) :=
